TargetSFI/CSTest.v
@@ -5,6 +5,11 @@ Require Import Coq.Lists.List. Import ListNotations.
 Require Import Coq.NArith.BinNat.
 Require Import Coq.ZArith.BinInt.
 Require Import Coq.Logic.Decidable.
+Require Import Coq.FSets.FMapInterface.
+Require Import Coq.FSets.FMapFacts.
+Require Import Coq.Init.Logic.
+
+Require Import Program.
 
 From QuickChick Require Import QuickChick.
 Import QcDefaultNotation. Import QcNotation. Open Scope qc_scope.
@@ -32,7 +37,177 @@ Proof.
     + apply instr_eq_dec.
   - auto.
 Defined.
-    
+
+Theorem step_Equal_1:
+  forall (g : Env.t) (mem1 mem2 mem': Memory.t)
+         (pc pc': RiscMachine.pc)
+         (regs regs' : RegisterFile.t) (t : trace) ,
+    BinNatMap.Equal mem1 mem2 ->
+    step g (mem1,pc,regs) t (mem',pc',regs') ->
+    step g (mem2,pc,regs) t (mem',pc',regs').
+Proof.
+  intros g mem1 mem2 mem' pc pc' regs reg' t Hmem1 Hstep.
+  
+  inversion Hstep; subst.
+  apply executing_equal with (m1:=mem1) (m2:=mem2) in H3.
+  apply Memory.Equal_sym in Hmem1.
+  apply Memory.Equal_trans with (m1:=mem2) (m2:=mem1) (m3:=mem') in H7. 
+  apply Nop. assumption. assumption. assumption. assumption.
+
+  apply executing_equal with (m1:=mem1) (m2:=mem2) in H4.
+  apply Memory.Equal_sym in Hmem1.
+  apply Memory.Equal_trans with (m1:=mem2) (m2:=mem1) (m3:=mem') in H8.
+  apply Const with (val:=val) (reg:=reg). assumption. reflexivity. assumption. assumption. assumption. 
+
+  apply executing_equal with (m1:=mem1) (m2:=mem2) in H5.
+  apply Memory.Equal_sym in Hmem1.
+  apply Memory.Equal_trans with (m1:=mem2) (m2:=mem1) (m3:=mem') in H9.
+  apply Mov with (reg_src:=reg_src) (reg_dst:=reg_dst) (val:=val). 
+  assumption. assumption. reflexivity. assumption. assumption. assumption.
+
+  apply executing_equal with (m1:=mem1) (m2:=mem2) in H6.
+  apply Memory.Equal_sym in Hmem1.
+  apply Memory.Equal_trans with (m1:=mem2) (m2:=mem1) (m3:=mem') in H10.
+  apply BinOp with (op:=op) (reg_src1:=reg_src1) (reg_src2:=reg_src2)
+                   (reg_dst:=reg_dst) (val1:=val1) (val2:=val2).
+  assumption.  assumption.  assumption. reflexivity.  assumption.  assumption.
+  assumption.
+
+  apply executing_equal with (m1:=mem1) (m2:=mem2) in H6.
+  apply Memory.Equal_sym in Hmem1.
+  apply Memory.Equal_trans with (m1:=mem2) (m2:=mem1) (m3:=mem') in H10.
+  apply Load with (rptr:=rptr) (rd:=rd) (ptr:=ptr) (val:=val).
+  assumption.  assumption.
+  rewrite H8.
+  apply Memory.get_value_Equal. apply Memory.Equal_sym. apply Hmem1.
+  reflexivity.  assumption. assumption.  assumption.
+
+  apply executing_equal with (m1:=mem1) (m2:=mem2) in H5.
+  apply Memory.Equal_sym in Hmem1.
+  apply Store with (rptr:=rptr) (rs:=rs) (ptr:=ptr) (val:=val). 
+  assumption. assumption. assumption.
+  apply Memory.set_value_Equal with (ptr:=(Memory.to_address ptr)) (val:=val) in Hmem1. 
+  apply Memory.Equal_trans with (m1:=(Memory.set_value mem2 (Memory.to_address ptr) val))
+                                (m2:=(Memory.set_value mem1 (Memory.to_address ptr) val))
+                                (m3:=mem').
+  assumption. assumption. assumption.
+
+  apply executing_equal with (m1:=mem1) (m2:=mem2) in H5.
+  apply Memory.Equal_sym in Hmem1.
+  apply Memory.Equal_trans with (m1:=mem2) (m2:=mem1) (m3:=mem') in H9.
+  apply BnzNZ with (reg:=reg) (val:=val).
+  assumption. assumption. assumption. assumption. assumption. assumption.
+
+  apply executing_equal with (m1:=mem1) (m2:=mem2) in H4.
+  apply Memory.Equal_sym in Hmem1.
+  apply Memory.Equal_trans with (m1:=mem2) (m2:=mem1) (m3:=mem') in H8.
+  apply BnzZ with (reg:=reg) (offset:=offset).
+  assumption. assumption. assumption. assumption. assumption.
+
+  apply executing_equal with (m1:=mem1) (m2:=mem2) in H6.
+  apply Memory.Equal_sym in Hmem1.
+  apply Memory.Equal_trans with (m1:=mem2) (m2:=mem1) (m3:=mem') in H10.
+  apply Return with (reg:=reg).
+  assumption. assumption. assumption. assumption. assumption.
+  assumption. assumption.
+
+  apply executing_equal with (m1:=mem1) (m2:=mem2) in H5.
+  apply Memory.Equal_sym in Hmem1.
+  apply Memory.Equal_trans with (m1:=mem2) (m2:=mem1) (m3:=mem') in H9.
+  apply Jump with (reg:=reg).
+  assumption. assumption. assumption. assumption. assumption.
+  assumption.
+
+  apply executing_equal with (m1:=mem1) (m2:=mem2) in H4.
+  apply Memory.Equal_sym in Hmem1.
+  apply Memory.Equal_trans with (m1:=mem2) (m2:=mem1) (m3:=mem') in H8.
+  apply Jal.
+  assumption. auto. 
+  assumption. assumption. assumption.
+
+  apply executing_equal with (m1:=mem1) (m2:=mem2) in H6.
+  apply Memory.Equal_sym in Hmem1.
+  apply Memory.Equal_trans with (m1:=mem2) (m2:=mem1) (m3:=mem') in H10.
+  apply Call. 
+  assumption. auto. 
+  assumption. assumption. assumption. assumption.
+  assumption.
+Qed.
+  
+Theorem step_Equal_2:
+  forall (g : Env.t) (mem mem1 mem2 : Memory.t)
+         (pc pc': RiscMachine.pc)
+         (regs regs' : RegisterFile.t) (t : trace) ,
+    BinNatMap.Equal mem1 mem2 ->
+    step g (mem,pc,regs) t (mem1,pc',regs') ->
+    step g (mem,pc,regs) t (mem2,pc',regs').
+Proof.
+  intros g mem mem1 mem2 pc pc' reg regs' t Hmem Hstep.
+  inversion Hstep; subst.
+  - (* Nop *)
+    apply Nop. assumption.
+    apply Memory.Equal_trans with (m1:=mem) (m2:=mem1) (m3:=mem2).
+    assumption. assumption.
+  - apply Const with (val:=val) (reg:=reg0).
+    assumption. reflexivity.
+    apply Memory.Equal_trans with (m1:=mem) (m2:=mem1) (m3:=mem2).
+    assumption. assumption.
+  - apply Mov with (reg_src:=reg_src) (reg_dst:=reg_dst) (val:=val).
+    assumption. assumption. reflexivity.
+    apply Memory.Equal_trans with (m1:=mem) (m2:=mem1) (m3:=mem2).
+    assumption. assumption.
+  - apply BinOp with (op:=op) (reg_src1:=reg_src1) (reg_src2:=reg_src2)
+                   (reg_dst:=reg_dst) (val1:=val1) (val2:=val2).
+    assumption. assumption. assumption. auto. 
+    apply Memory.Equal_trans with (m1:=mem) (m2:=mem1) (m3:=mem2).
+    assumption. assumption.
+  - apply Load with (rptr:=rptr) (rd:=rd) (ptr:=ptr) (val:=val).
+    assumption. assumption. auto. reflexivity.
+    apply Memory.Equal_trans with (m1:=mem) (m2:=mem1) (m3:=mem2). assumption. assumption. 
+  - apply Store with (rptr:=rptr) (rs:=rs) (ptr:=ptr) (val:=val).
+    assumption. assumption. assumption.
+    apply Memory.Equal_trans with (m1:= (Memory.set_value mem (Memory.to_address ptr) val))
+                                  (m2:=mem1) (m3:=mem2). assumption. assumption.
+  - apply BnzNZ with (reg:=reg0) (val:=val).
+    assumption. assumption. assumption. 
+    apply Memory.Equal_trans with (m1:=mem) (m2:=mem1) (m3:=mem2). assumption. assumption. 
+  - apply BnzZ with (reg:=reg0) (offset:=offset).
+    assumption. assumption.
+    apply Memory.Equal_trans with (m1:=mem) (m2:=mem1) (m3:=mem2). assumption. assumption. 
+  - apply Return with (reg:=reg0).
+    assumption. assumption. assumption. assumption. 
+    apply Memory.Equal_trans with (m1:=mem) (m2:=mem1) (m3:=mem2). assumption. assumption.
+  - apply Jump with (reg:=reg0).
+    assumption. assumption. assumption. 
+    apply Memory.Equal_trans with (m1:=mem) (m2:=mem1) (m3:=mem2). assumption. assumption.
+  - apply Jal.
+    assumption. auto.
+    apply Memory.Equal_trans with (m1:=mem) (m2:=mem1) (m3:=mem2). assumption. assumption.
+  - apply Call. 
+    assumption. auto. assumption. assumption.
+    apply Memory.Equal_trans with (m1:=mem) (m2:=mem1) (m3:=mem2). assumption. assumption.
+Qed.
+
+
+Ltac exec_contra H :=
+  match goal with
+  | [ H1 : executing _ _ _ |- _] =>
+    unfold executing in H1; rewrite H in H1; inversion H1
+  end.
+
+Ltac mem_contra Hmem :=
+  match goal with
+  | [ H1 : Memory.Equal _ _ |- _ ] =>
+    apply Memory.eqb_Equal in H1; rewrite Hmem in H1; inversion H1
+  end.
+
+Ltac right_inv := right; intro contra; inversion contra; subst.
+
+Ltac inc_pc_contra H Hpc :=
+  right_inv;
+  try (rewrite N.eqb_refl in Hpc; inversion Hpc);
+  exec_contra H.
+
 Instance step_dec(g : Env.t) (st : MachineState.t) (t : trace)
          (st' : MachineState.t): Dec (step g st t st'). 
 Proof.
@@ -41,24 +216,225 @@ Proof.
   destruct st' as [[mem' pc'] gen_regs'].
   destruct (Memory.get_word mem pc) eqn:H.
   - destruct w.
-    + right. unfold not. intro H1. inversion H1.
-      * unfold executing in H5. subst. rewrite H in H5. auto.
-      * unfold executing in H5. subst. rewrite H in H5. auto.
-      * unfold executing in H6. subst. rewrite H in H6. auto.
-      * unfold executing in H7. subst. rewrite H in H7. auto.
-      * unfold executing in H7. subst. rewrite H in H7. auto.
-      * unfold executing in H7. subst. rewrite H in H7. auto.
-      * unfold executing in H6. subst. rewrite H in H6. auto.
-      * unfold executing in H6. subst. rewrite H in H6. auto.
-      * unfold executing in H7. subst. rewrite H in H7. auto.
-      * unfold executing in H6. subst. rewrite H in H6. auto.
-      * unfold executing in H5. subst. rewrite H in H5. auto.
-      * unfold executing in H7. subst. rewrite H in H7. auto.
-    + destruct t0.
-      * destruct (N.eqb pc' (inc_pc pc)) eqn:Hpc. rewrite N.eqb_eq in Hpc.
-        rewrite Hpc. destruct (gen_regs = gen_regs') eqn:Hregs.
-        left. apply Nop.
+    + right. unfold not. intro H1.
+      inversion H1;
+        try ( match goal with
+              | H' : executing _ _ _ |- _ =>
+                unfold executing in H'; subst; rewrite H in H'; auto
+              end
+            ).
+    + destruct i as [|val reg|rs rd|op rs1 rs2 rd|rptr rd|rptr rs|r im|r|addr|].
+      * (* INop *)
+        destruct (Memory.eqb mem mem') eqn:Hmem.
+        { (* mem = mem' *)
+          apply Memory.eqb_Equal in Hmem.
+          destruct t0.
+          { (* empty trace *)
+            destruct (N.eqb pc' (inc_pc pc)) eqn:Hpc.
+            { (* pc' = pc+1 *)
+              rewrite N.eqb_eq in Hpc. rewrite Hpc.
+              destruct (RegisterFile.eqb gen_regs gen_regs') eqn:Hregs.
+              { (* regs=regs'*)
+                apply RegisterFile.eqb_eq in Hregs. rewrite Hregs.
+                left. subst. apply Nop.
+                unfold executing. rewrite H. reflexivity. assumption. 
+              }
+              { (* regs <> regs' *)
+                right_inv;
+                try ( apply RegisterFile.neqb_neq in Hregs;
+                      apply Hregs; reflexivity);
+                exec_contra H.
+              }
+            }
+            { (* pc' <> pc+1 *) inc_pc_contra H Hpc. }
+          }
+          { (* non empty trace *) right_inv; exec_contra H. }
+        }
+        { (* mem <> mem' *) right_inv; try (mem_contra Hmem); exec_contra H. }
+      * (* IConst *)
+        destruct (Memory.eqb mem mem') eqn:Hmem.
+        { (* mem = mem' *)
+          apply Memory.eqb_Equal in Hmem.
+          destruct t0.
+          { (* empty trace *)
+            destruct (N.eqb pc' (inc_pc pc)) eqn:Hpc.
+            { (* pc' = pc+1 *)
+              rewrite N.eqb_eq in Hpc. rewrite Hpc.
+              destruct (RegisterFile.eqb
+                          (RegisterFile.set_register reg val gen_regs)
+                          gen_regs') eqn:Hregs.
+              { (* regs[r<reg-val]=regs'*)                
+                left. apply Const with (val:=val) (reg:=reg).
+                unfold executing. rewrite H. auto.
+                apply RegisterFile.eqb_eq. assumption. assumption. 
+              }
+              { (* regs[r<reg-val] <> regs' *)
+                right_inv; try (exec_contra H);
+                try ( apply RegisterFile.neqb_neq in Hregs;
+                      apply Hregs; reflexivity).
+                subst. 
+                rewrite RegisterFile.eqb_refl with
+                    (regs:=(RegisterFile.set_register reg val gen_regs)) in Hregs.
+                inversion Hregs. 
+              }
+            }
+            {  inc_pc_contra H Hpc. }
+          }
+          { (* non empty trace *)  right_inv; exec_contra H. }
+        }
+        { (* mem <> mem' *)  right_inv; try (mem_contra Hmem); exec_contra H. }
+
+      * (* IMov *)
+        destruct (Memory.eqb mem mem') eqn:Hmem.
+        { (* mem = mem' *)
+          apply Memory.eqb_Equal in Hmem.
+          destruct t0.
+          { (* empty trace *)
+            destruct (N.eqb pc' (inc_pc pc)) eqn:Hpc.
+            { (* pc' = pc+1 *)
+              rewrite N.eqb_eq in Hpc. rewrite Hpc.
+              destruct (RegisterFile.get_register rs gen_regs) eqn:Hval.
+              { (* RegisterFile.get_register rs gen_regs = Some v *)               
+                destruct (RegisterFile.eqb
+                            (RegisterFile.set_register rd v gen_regs)
+                            gen_regs') eqn:Hregs.
+                { (* regs[rd<-v]=regs'*)                
+                  left.
+                  apply Mov with (reg_src:=rs) (reg_dst:=rd) (val:=v). 
+                  unfold executing. rewrite H. auto.
+                  symmetry. assumption. 
+                  apply RegisterFile.eqb_eq. assumption. assumption. 
+                }
+                { (* regs[rd<-d] <> regs' *)
+                  right_inv; try (exec_contra H).
+                  subst.
+                  rewrite Hval in H6. inversion H6. subst. 
+                  rewrite RegisterFile.eqb_refl with
+                      (regs:= (RegisterFile.set_register rd v gen_regs)) in Hregs.
+                  inversion Hregs. 
+                }                
+              }
+              { (* RegisterFile.get_register rs gen_regs = None *)
+                right_inv; try(exec_contra H).
+                subst. rewrite Hval in H6. inversion H6. 
+              }
+            }
+            { (* pc' <> pc+1 *)  inc_pc_contra H Hpc. }
+          }
+          { (* non empty trace *) right_inv; exec_contra H. }
+        }
+        { (* mem <> mem' *)  right_inv; try (mem_contra Hmem); exec_contra H. }
+        
+      *  (* IBinOp *)
+        destruct (Memory.eqb mem mem') eqn:Hmem.
+        { (* mem = mem' *)
+          apply Memory.eqb_Equal in Hmem.
+          destruct t0.
+          { (* empty trace *)
+            destruct (N.eqb pc' (inc_pc pc)) eqn:Hpc.
+            { (* pc' = pc+1 *)
+              rewrite N.eqb_eq in Hpc. rewrite Hpc.
+              destruct (RegisterFile.get_register rs1 gen_regs) eqn:Hval1. rename v into v1.
+              { (* RegisterFile.get_register rs gen_regs = Some v1 *)
+                destruct (RegisterFile.get_register rs2 gen_regs) eqn:Hval2. rename v into v2.
+                { (* RegisterFile.get_register rs2 gen_regs = Some v2 *)
+                  destruct (RegisterFile.eqb
+                            (RegisterFile.set_register rd (executing_binop op v1 v2) gen_regs)
+                            gen_regs') eqn:Hregs.
+                  { (* regs[rd<-v1 binop v2]=regs'*)                
+                    left.
+                    apply BinOp with (op:=op) (reg_src1:=rs1) (reg_src2:=rs2)
+                                     (reg_dst:=rd) (val1:=v1) (val2:=v2).
+                    unfold executing. rewrite H. reflexivity.
+                    symmetry. assumption. symmetry. assumption. 
+                    apply RegisterFile.eqb_eq. assumption. assumption. 
+                  }
+                  { (* regs[rd<-v1 binop v2]<>regs' *)
+                    right_inv; try (exec_contra H).
+                    subst.
+                    rewrite Hval1 in H6. inversion H6.
+                    rewrite Hval2 in H7. inversion H7. subst.
+                    subst result. 
+                    rewrite RegisterFile.eqb_refl with
+                        (regs:=  (RegisterFile.set_register rd
+                                                            (executing_binop op v1 v2)
+                                                            gen_regs)) in Hregs.
+                    inversion Hregs. 
+                  }                
+                }
+                { (* RegisterFile.get_register rs2 gen_regs = None *)
+                  right_inv; try(exec_contra H).
+                  subst. rewrite Hval2 in H7. inversion H7. 
+                }
+              }
+              { (* RegisterFile.get_register rs1 gen_regs = None *)
+                right_inv; try(exec_contra H).
+                subst. rewrite Hval1 in H6. inversion H6. 
+              }
+            }
+            { (* pc' <> pc+1 *)  inc_pc_contra H Hpc. }
+          }
+          { (* non empty trace *) right_inv; exec_contra H. }
+        }
+        { (* mem <> mem' *)  right_inv; try (mem_contra Hmem); exec_contra H. }
+
+      * (* ILoad *) 
+        destruct (Memory.eqb mem mem') eqn:Hmem.
+        { (* mem = mem' *)
+          apply Memory.eqb_Equal in Hmem.
+          destruct t0.
+          { (* empty trace *)
+            destruct (N.eqb pc' (inc_pc pc)) eqn:Hpc.
+            { (* pc' = pc+1 *)
+              rewrite N.eqb_eq in Hpc. rewrite Hpc.
+              destruct (RegisterFile.get_register rptr gen_regs) eqn:Hptr.  
+              { (* RegisterFile.get_register rd gen_regs = Some ptr *)
+                rename v into ptr.
+                destruct (Memory.get_value mem (Memory.to_address ptr)) eqn:Hval.
+                { (* Memory.get_value mem (Memory.to_address ptr) = Some val *)
+                  rename v into val. 
+                  destruct (RegisterFile.eqb
+                            (RegisterFile.set_register rd val gen_regs)
+                            gen_regs') eqn:Hregs.
+                  { (* regs[rd<-val]=regs'*)                
+                    left.
+                    apply Load with (rptr:=rptr) (rd:=rd) (ptr:=ptr) (val:=val).
+                    unfold executing. rewrite H. auto.
+                    symmetry. assumption. symmetry. assumption.  
+                    apply RegisterFile.eqb_eq. assumption. assumption. 
+                  }
+                  { (* regs[rd<-d] <> regs' *)
+                    right_inv; try (exec_contra H).
+                    subst.
+                    subst addr.
+                    rewrite <- H6 in Hptr. inversion Hptr. subst. 
+                    rewrite Hval in H7. inversion H7. subst. 
+                    rewrite RegisterFile.eqb_refl with
+                        (regs:= (RegisterFile.set_register rd val gen_regs)) in Hregs.
+                    inversion Hregs. 
+                  }                
+                }
+                { (* Memory.get_value mem (Memory.to_address ptr) = None *)
+                  right_inv; try(exec_contra H). subst.
+                  rewrite <- H6 in Hptr. inversion Hptr. subst. subst addr.
+                  rewrite <- H7 in Hval. inversion Hval.  
+                }
+              }
+              { (* RegisterFile.get_register rd gen_regs = None *)
+                right_inv; try(exec_contra H). subst.
+                rewrite Hptr in H6. inversion H6. 
+              }
+            }
+            { (* pc' <> pc+1 *)  inc_pc_contra H Hpc. }
+          }
+          { (* non empty trace *) right_inv; exec_contra H. }
+        }
+        { (* mem <> mem' *)  right_inv; try (mem_contra Hmem); exec_contra H. }
+
+      * (* Store *)
+        
       Admitted.
+
 
 Definition eqb_event (e1 e2: event) : bool :=
   match (e1,e2) with
